Progress #4

rocq-skylabs-brick/tests/float_support.v
@@ -11,6 +11,8 @@ Require Import skylabs.lang.cpp.semantics.genv.
 Require Import skylabs.lang.cpp.semantics.values.
 Require Import skylabs.lang.cpp.semantics.cast.
 Require Import skylabs.lang.cpp.semantics.cast_operator.
+Require Import skylabs.lang.cpp.semantics.operator.
+Require Import skylabs.lang.cpp.logic.raw.
 
 Open Scope pstring_scope.
 Open Scope Z_scope.
@@ -99,6 +101,26 @@ Example convert_type_accepts_float_double_add tu :
   convert_type_op tu Badd Tfloat Tdouble = Some (Tdouble, Tdouble, Tdouble).
 Proof. reflexivity. Qed.
 
+Example convert_type_accepts_double_float_add tu :
+  convert_type_op tu Badd Tdouble Tfloat = Some (Tdouble, Tdouble, Tdouble).
+Proof. reflexivity. Qed.
+
+Example convert_type_accepts_float_int_add tu :
+  convert_type_op tu Badd Tfloat Tint = Some (Tfloat, Tfloat, Tfloat).
+Proof. reflexivity. Qed.
+
+Example convert_type_accepts_int_double_add tu :
+  convert_type_op tu Badd Tint Tdouble = Some (Tdouble, Tdouble, Tdouble).
+Proof. reflexivity. Qed.
+
+Example convert_type_accepts_float_double_compare tu :
+  convert_type_op tu Blt Tfloat Tdouble = Some (Tdouble, Tdouble, Tbool).
+Proof. reflexivity. Qed.
+
+Example convert_type_accepts_int_double_compare tu :
+  convert_type_op tu Bge Tint Tdouble = Some (Tdouble, Tdouble, Tbool).
+Proof. reflexivity. Qed.
+
 Example convert_rejects_unsupported_float_to_int {σ : genv} tu v v' :
   @convert σ tu Tlongdouble Tint v v' = False.
 Proof. reflexivity. Qed.
@@ -111,6 +133,13 @@ Definition f32_inf : fp_carrier Ffloat := fp_of_bits Ffloat 2139095040%Z.
 Definition f64_inf : fp_carrier Fdouble := fp_of_bits Fdouble 9218868437227405312%Z.
 Definition f32_nan : fp_carrier Ffloat := fp_default_nan Ffloat.
 Definition f64_nan : fp_carrier Fdouble := fp_default_nan Fdouble.
+Definition f32_nan_payload : fp_carrier Ffloat := fp_of_bits Ffloat 2143289345%Z.
+Definition f64_nan_payload : fp_carrier Fdouble := fp_of_bits Fdouble 9221120237041090561%Z.
+
+Definition little_float_test_genv : genv :=
+  {| genv_tu := empty_tu (abi.mkT int_rank.Ilong Signed Signed Little) |}.
+Definition big_float_test_genv : genv :=
+  {| genv_tu := empty_tu (abi.mkT int_rank.Ilong Signed Signed Big) |}.
 
 Example has_type_prop_float_value {σ : genv} :
   has_type_prop (Vfloat_ Ffloat f32_one) Tfloat.
@@ -187,6 +216,38 @@ Proof. vm_compute. reflexivity. Qed.
 Example double_nan_compare_unordered : fp_compare Fdouble f64_nan f64_nan = None.
 Proof. vm_compute. reflexivity. Qed.
 
+Example default_nan_bits_float :
+  fp_to_bits Ffloat (fp_default_nan Ffloat) = 2143289344%Z.
+Proof. apply fp_to_bits_default_nan_Ffloat. Qed.
+
+Example default_nan_bits_double :
+  fp_to_bits Fdouble (fp_default_nan Fdouble) = 9221120237041090560%Z.
+Proof. apply fp_to_bits_default_nan_Fdouble. Qed.
+
+Example fp32_nan_payload_bits_preserved :
+  fp_to_bits Ffloat (fp_of_bits Ffloat 2143289345%Z) = 2143289345%Z.
+Proof. apply fp_to_of_bits_Ffloat. change (0 <= 2143289345 < 4294967296)%Z. lia. Qed.
+
+Example fp64_nan_payload_bits_preserved :
+  fp_to_bits Fdouble (fp_of_bits Fdouble 9221120237041090561%Z) = 9221120237041090561%Z.
+Proof. apply fp_to_of_bits_Fdouble. change (0 <= 9221120237041090561 < 18446744073709551616)%Z. lia. Qed.
+
+Example float_nan_add_canonical_bits :
+  fp_to_bits Ffloat (fp_add Ffloat f32_nan f32_one) = 2143289344%Z.
+Proof. vm_compute. reflexivity. Qed.
+
+Example double_nan_add_canonical_bits :
+  fp_to_bits Fdouble (fp_add Fdouble f64_nan f64_one) = 9221120237041090560%Z.
+Proof. vm_compute. reflexivity. Qed.
+
+Example float_nan_neg_canonical_bits :
+  fp_to_bits Ffloat (fp_neg Ffloat f32_nan) = 2143289344%Z.
+Proof. vm_compute. reflexivity. Qed.
+
+Example double_nan_neg_canonical_bits :
+  fp_to_bits Fdouble (fp_neg Fdouble f64_nan) = 9221120237041090560%Z.
+Proof. vm_compute. reflexivity. Qed.
+
 Example float_nan_eq_false :
   (if fp_compare Ffloat f32_nan f32_nan is Some Eq then true else false) = false.
 Proof. vm_compute. reflexivity. Qed.
@@ -197,6 +258,18 @@ Proof. vm_compute. reflexivity. Qed.
 
 Example float_nan_ordered_lt_false :
   (if fp_compare Ffloat f32_nan f32_nan is Some Lt then true else false) = false.
+Proof. vm_compute. reflexivity. Qed.
+
+Example double_nan_eq_false :
+  (if fp_compare Fdouble f64_nan f64_nan is Some Eq then true else false) = false.
+Proof. vm_compute. reflexivity. Qed.
+
+Example double_nan_neq_true :
+  (if fp_compare Fdouble f64_nan f64_nan is Some Eq then false else true) = true.
+Proof. vm_compute. reflexivity. Qed.
+
+Example double_nan_ordered_lt_false :
+  (if fp_compare Fdouble f64_nan f64_nan is Some Lt then true else false) = false.
 Proof. vm_compute. reflexivity. Qed.
 
 Example conv_float_identity_example {σ : genv} tu :
@@ -230,3 +303,165 @@ Proof.
   eapply ConvFloatToInt; [reflexivity|reflexivity|vm_compute; reflexivity|].
   rewrite -has_int_type /bitsize.bound /bitsize.min_val /bitsize.max_val /=; lia.
 Qed.
+
+Example eval_add_mixed_float_double_after_conversion {σ : genv} tu :
+  eval_binop_pure tu Badd Tdouble Tdouble Tdouble
+    (Vfloat_ Fdouble (fp_float_to_double f32_one))
+    (Vfloat_ Fdouble f64_one)
+    (Vfloat_ Fdouble (fp_add Fdouble (fp_float_to_double f32_one) f64_one)).
+Proof. apply eval_add_float. reflexivity. Qed.
+
+Example eval_cmp_mixed_float_double_after_conversion {σ : genv} tu :
+  eval_binop_pure tu Blt Tdouble Tdouble Tbool
+    (Vfloat_ Fdouble (fp_float_to_double f32_one))
+    (Vfloat_ Fdouble f64_one)
+    (Vbool (fp_cmp_result (fp_compare Fdouble (fp_float_to_double f32_one) f64_one) Blt)).
+Proof. apply eval_cmp_float; [tauto|reflexivity]. Qed.
+
+Example raw_bytes_float32_intro {σ : genv} :
+  raw_bytes_of_val σ Tfloat (Vfloat_ Ffloat f32_one) (fp_raw_bytes σ Ffloat f32_one).
+Proof. apply raw_bytes_of_val_float_intro. reflexivity. Qed.
+
+Example raw_bytes_float64_intro {σ : genv} :
+  raw_bytes_of_val σ Tdouble (Vfloat_ Fdouble f64_one) (fp_raw_bytes σ Fdouble f64_one).
+Proof. apply raw_bytes_of_val_float_intro. reflexivity. Qed.
+
+Example raw_bytes_float32_length {σ : genv} :
+  length (fp_raw_bytes σ Ffloat f32_one) = 4%nat.
+Proof. rewrite fp_raw_bytes_length. reflexivity. Qed.
+
+Example raw_bytes_float64_length {σ : genv} :
+  length (fp_raw_bytes σ Fdouble f64_one) = 8%nat.
+Proof. rewrite fp_raw_bytes_length. reflexivity. Qed.
+
+Example raw_bytes_float32_one_little_endian :
+  fp_raw_bytes little_float_test_genv Ffloat f32_one =
+  raw_int_byte <$> [0%N; 0%N; 128%N; 63%N].
+Proof.
+  rewrite /fp_raw_bytes z_to_bytes._Z_to_bytes_eq /z_to_bytes._Z_to_bytes_def /z_to_bytes._Z_to_bytes_le
+    /z_to_bytes._Z_to_bytes_unsigned_le /z_to_bytes._Z_to_bytes_unsigned_le' /=.
+  reflexivity.
+Qed.
+
+Example raw_bytes_float32_one_big_endian :
+  fp_raw_bytes big_float_test_genv Ffloat f32_one =
+  raw_int_byte <$> [63%N; 128%N; 0%N; 0%N].
+Proof.
+  rewrite /fp_raw_bytes z_to_bytes._Z_to_bytes_eq /z_to_bytes._Z_to_bytes_def /z_to_bytes._Z_to_bytes_le
+    /z_to_bytes._Z_to_bytes_unsigned_le /z_to_bytes._Z_to_bytes_unsigned_le' /=.
+  reflexivity.
+Qed.
+
+Example raw_bytes_float64_one_little_endian :
+  fp_raw_bytes little_float_test_genv Fdouble f64_one =
+  raw_int_byte <$> [0%N; 0%N; 0%N; 0%N; 0%N; 0%N; 240%N; 63%N].
+Proof.
+  rewrite /fp_raw_bytes z_to_bytes._Z_to_bytes_eq /z_to_bytes._Z_to_bytes_def /z_to_bytes._Z_to_bytes_le
+    /z_to_bytes._Z_to_bytes_unsigned_le /z_to_bytes._Z_to_bytes_unsigned_le' /=.
+  reflexivity.
+Qed.
+
+Example raw_bytes_float64_one_big_endian :
+  fp_raw_bytes big_float_test_genv Fdouble f64_one =
+  raw_int_byte <$> [63%N; 240%N; 0%N; 0%N; 0%N; 0%N; 0%N; 0%N].
+Proof.
+  rewrite /fp_raw_bytes z_to_bytes._Z_to_bytes_eq /z_to_bytes._Z_to_bytes_def /z_to_bytes._Z_to_bytes_le
+    /z_to_bytes._Z_to_bytes_unsigned_le /z_to_bytes._Z_to_bytes_unsigned_le' /=.
+  reflexivity.
+Qed.
+
+Example raw_bytes_float32_same_bytes_same_value {σ : genv} rs f :
+  raw_bytes_of_val σ Tfloat (Vfloat_ Ffloat f32_one) rs ->
+  raw_bytes_of_val σ Tfloat (Vfloat_ Ffloat f) rs ->
+  f = f32_one.
+Proof.
+  intros H1 H2.
+  symmetry. eapply raw_bytes_of_val_float_unique_val; [reflexivity|exact H1|exact H2].
+Qed.
+
+Example raw_bytes_float64_same_bytes_same_value {σ : genv} rs f :
+  raw_bytes_of_val σ Tdouble (Vfloat_ Fdouble f64_one) rs ->
+  raw_bytes_of_val σ Tdouble (Vfloat_ Fdouble f) rs ->
+  f = f64_one.
+Proof.
+  intros H1 H2.
+  symmetry. eapply raw_bytes_of_val_float_unique_val; [reflexivity|exact H1|exact H2].
+Qed.
+
+Example raw_bytes_float32_nan_payload_survives_roundtrip {σ : genv} rs f :
+  raw_bytes_of_val σ Tfloat (Vfloat_ Ffloat f32_nan_payload) rs ->
+  raw_bytes_of_val σ Tfloat (Vfloat_ Ffloat f) rs ->
+  fp_to_bits Ffloat f = 2143289345%Z.
+Proof.
+  intros H1 H2.
+  assert (f = f32_nan_payload) as ->.
+  { symmetry. eapply raw_bytes_of_val_float_unique_val; [reflexivity|exact H1|exact H2]. }
+  apply fp_to_of_bits_Ffloat. change (0 <= 2143289345 < 4294967296)%Z. lia.
+Qed.
+
+Example raw_bytes_float64_nan_payload_survives_roundtrip {σ : genv} rs f :
+  raw_bytes_of_val σ Tdouble (Vfloat_ Fdouble f64_nan_payload) rs ->
+  raw_bytes_of_val σ Tdouble (Vfloat_ Fdouble f) rs ->
+  fp_to_bits Fdouble f = 9221120237041090561%Z.
+Proof.
+  intros H1 H2.
+  assert (f = f64_nan_payload) as ->.
+  { symmetry. eapply raw_bytes_of_val_float_unique_val; [reflexivity|exact H1|exact H2]. }
+  apply fp_to_of_bits_Fdouble. change (0 <= 9221120237041090561 < 18446744073709551616)%Z. lia.
+Qed.
+
+Section raw_byte_reinterpretation_tests.
+  Context `{Σ : cpp_logic} {σ : genv}.
+
+  Example raw_bytes_float32_to_unsigned_bits :
+    raw_bytes_of_val σ Tuint (Vint (fp_to_bits Ffloat f32_one)) (fp_raw_bytes σ Ffloat f32_one).
+  Proof.
+    apply Endian.raw_bytes_of_val_float_to_unsigned_bits; reflexivity.
+  Qed.
+
+  Example raw_bytes_float64_to_unsigned_bits :
+    raw_bytes_of_val σ Tulonglong (Vint (fp_to_bits Fdouble f64_one)) (fp_raw_bytes σ Fdouble f64_one).
+  Proof.
+    apply Endian.raw_bytes_of_val_float_to_unsigned_bits; reflexivity.
+  Qed.
+
+  Example raw_bytes_unsigned_bits_to_float32 rs :
+    raw_bytes_of_val σ Tuint (Vint (fp_to_bits Ffloat f32_one)) rs ->
+    raw_bytes_of_val σ Tfloat (Vfloat_ Ffloat f32_one) rs.
+  Proof.
+    intros Hraw.
+    rewrite -(fp_of_to_bits Ffloat f32_one).
+    eapply (@raw_bytes_of_val_unsigned_bits_to_float σ int_rank.Iint Ffloat (fp_to_bits Ffloat f32_one) rs);
+      [reflexivity|reflexivity|exact Hraw].
+  Qed.
+
+  Example raw_bytes_unsigned_bits_to_float64 rs :
+    raw_bytes_of_val σ Tulonglong (Vint (fp_to_bits Fdouble f64_one)) rs ->
+    raw_bytes_of_val σ Tdouble (Vfloat_ Fdouble f64_one) rs.
+  Proof.
+    intros Hraw.
+    rewrite -(fp_of_to_bits Fdouble f64_one).
+    eapply (@raw_bytes_of_val_unsigned_bits_to_float σ int_rank.Ilonglong Fdouble (fp_to_bits Fdouble f64_one) rs);
+      [reflexivity|reflexivity|exact Hraw].
+  Qed.
+
+  Example raw_bytes_unsigned_nan_payload_to_float32 rs :
+    raw_bytes_of_val σ Tuint (Vint 2143289345%Z) rs ->
+    raw_bytes_of_val σ Tfloat (Vfloat_ Ffloat f32_nan_payload) rs.
+  Proof.
+    intros Hraw.
+    change (Vfloat_ Ffloat f32_nan_payload) with (Vfloat_ Ffloat (fp_of_bits Ffloat 2143289345%Z)).
+    eapply (@raw_bytes_of_val_unsigned_bits_to_float σ int_rank.Iint Ffloat 2143289345%Z rs);
+      [reflexivity|reflexivity|exact Hraw].
+  Qed.
+
+  Example raw_bytes_unsigned_nan_payload_to_float64 rs :
+    raw_bytes_of_val σ Tulonglong (Vint 9221120237041090561%Z) rs ->
+    raw_bytes_of_val σ Tdouble (Vfloat_ Fdouble f64_nan_payload) rs.
+  Proof.
+    intros Hraw.
+    change (Vfloat_ Fdouble f64_nan_payload) with (Vfloat_ Fdouble (fp_of_bits Fdouble 9221120237041090561%Z)).
+    eapply (@raw_bytes_of_val_unsigned_bits_to_float σ int_rank.Ilonglong Fdouble 9221120237041090561%Z rs);
+      [reflexivity|reflexivity|exact Hraw].
+  Qed.
+End raw_byte_reinterpretation_tests.
